Add wfo_sim and anywfo

nola/util/wfo.v
@@ -1,6 +1,6 @@
 (** * Equip types with a well-founded order *)
 
-From nola Require Import prelude.
+From nola Require Import prelude util.pred.
 From stdpp Require Export well_founded.
 Import EqNotations.
 
@@ -19,10 +19,12 @@ Arguments wfo_car : simpl never.
 Arguments wfo_lt {A} _ _ : simpl never, rename.
 Arguments wfo_lt_wf {A} : simpl never, rename.
 Infix "≺" := wfo_lt (at level 70, no associativity) : nola_scope.
+Notation "(≺)" := wfo_lt (only parsing) : nola_scope.
 
 (** Inverse of [≺] *)
 Definition wfo_gt {A : wfo} (a b : A) := b ≺ a.
 Infix "≻" := wfo_gt (at level 70, no associativity) : nola_scope.
+Notation "(≻)" := wfo_gt (only parsing) : nola_scope.
 
 (** [≺] is irreflexive *)
 Lemma wfo_lt_irrefl {A : wfo} (a : A) : ¬ a ≺ a.
@@ -71,3 +73,141 @@ Section sigT_wfo.
 
   Canonical sigT_wfo := Wfo (sigT F) sigT_lt sigT_lt_wf.
 End sigT_wfo.
+
+(** ** [≼*]: Simulation between [wfo]s *)
+
+(** Generator for [wfo_sim] *)
+Definition wfo_sim_gen {A B : wfo} (self : A * B → Prop) (ab : A * B) :=
+  let '(a, b) := ab in ∀ a', a' ≺ a → ∃ b', b' ≺ b ∧ self (a', b').
+
+(** [wfo_sim_gen] is monotone *)
+#[export] Instance wfo_sim_gen_mono A B : Mono1 (@wfo_sim_gen A B).
+Proof.
+  move=> φ ψ φψ [a b]/= W a' a'a. move: (W a' a'a)=> [b' [b'b /φψ ψa'b']].
+  by exists b'.
+Qed.
+
+(** [≼*]: Simulation between [wfo]s *)
+Definition wfo_sim {A B : wfo} (a : A) (b : B) : Prop := nu wfo_sim_gen (a, b).
+Infix "≼*" := wfo_sim (at level 70, no associativity) : nola_scope.
+
+(** Fold [≼*] *)
+Lemma wfo_sim_fold {A B : wfo} (a : A) (b : B) :
+  (∀ a', a' ≺ a → ∃ b', b' ≺ b ∧ a' ≼* b') → a ≼* b.
+Proof. move=> ?. by apply nu_fold. Qed.
+
+(** Unfold [≼*] *)
+Lemma wfo_sim_unfold {A B : wfo} (a : A) (b : B) :
+  a ≼* b → ∀ a', a' ≺ a → ∃ b', b' ≺ b ∧ a' ≼* b'.
+Proof. move=> asb. by apply nu_unfold in asb. Qed.
+
+(** Prove [≼*] by coinduction *)
+Lemma wfo_sim_coind {A B : wfo} (φ : A → B → Prop) :
+  (∀ a b, φ a b → (∀ a', a' ≺ a → ∃ b', b' ≺ b ∧ φ a' b')) →
+  ∀ a b, φ a b → a ≼* b.
+Proof.
+  move=> CH a b φab. apply (nu_coind (uncurry φ)); [|done]. clear a b φab.
+  move=> [a b]/= φab. by apply CH.
+Qed.
+
+(** Get [≼*] out of a monotone function *)
+Lemma wfo_sim_fun {A B : wfo} (f : A → B) :
+  (∀ a a', a' ≺ a → f a' ≺ f a) → ∀ a, a ≼* f a.
+Proof.
+  move=> fmono a. apply (wfo_sim_coind (λ a b, b = f a)); [|done]. clear a.
+  move=> a _ -> a' a'a. exists (f a'). split; [by apply fmono|done].
+Qed.
+
+(** [≼*] is reflexive *)
+#[export] Instance wfo_sim_refl {A : wfo} : Reflexive (@wfo_sim A A).
+Proof. move=> a. by apply (wfo_sim_fun id). Qed.
+
+(** [≼*] is transitive *)
+Lemma wfo_sim_trans {A B C : wfo} (a : A) (b : B) (c : C) :
+  a ≼* b → b ≼* c → a ≼* c.
+Proof.
+  move=> ab bc.
+  apply (wfo_sim_coind (λ a c, ∃ (b : B), a ≼* b ∧ b ≼* c)); [|by exists b].
+  clear. move=> a c [b [/wfo_sim_unfold ab /wfo_sim_unfold bc]] a' a'a.
+  move: {ab}(ab a' a'a)=> [b' [b'b a'sb']].
+  move: {bc}(bc b' b'b)=> [c' [c'c b'sc']].
+  exists c'. split; [done|]. by exists b'.
+Qed.
+
+(** [≺*]: [≼*] composed with [≺] *)
+Definition wfo_sim_lt {A B : wfo} (a : A) (b : B) : Prop :=
+  ∃ b', a ≼* b' ∧ b' ≺ b.
+Infix "≺*" := wfo_sim_lt (at level 70, no associativity) : nola_scope.
+
+(** Turn [≺] into [≺*] *)
+Lemma wfo_lt_to_sim_lt {A : wfo} (a b : A) : a ≺ b → a ≺* b.
+Proof. move=> ab. exists a. split; [by apply wfo_sim_refl|done]. Qed.
+
+(** Compose [≼*] and [≺*] *)
+Lemma wfo_sim_sim_lt_trans {A B C : wfo} (a : A) (b : B) (c : C) :
+  a ≼* b → b ≺* c → a ≺* c.
+Proof.
+  move=> asb [c' [bsc' c'c]]. exists c'. split; [|done].
+  by eapply wfo_sim_trans.
+Qed.
+
+(** Compose [≺*] and [≼*] *)
+Lemma wfo_sim_lt_sim_trans {A B C : wfo} (a : A) (b : B) (c : C) :
+  a ≺* b → b ≼* c → a ≺* c.
+Proof.
+  move=> [b' [asb' b'b]] /wfo_sim_unfold bsc.
+  move: {bsc}(bsc b' b'b)=> [c' [c'c b'sc']]. exists c'. split; [|done].
+  by eapply wfo_sim_trans.
+Qed.
+
+(** Turn [≼*] into [≺*] assuming transitivity of the target *)
+Lemma wfo_sim_to_sim_lt {A B : wfo} `{Transitive _ B.(wfo_lt)}
+  (a : A) (b : B) : a ≺* b → a ≼* b.
+Proof.
+  move=> [b' [/wfo_sim_unfold asb' b'b]]. apply wfo_sim_fold=> a' a'a.
+  move: {asb'}(asb' a' a'a)=> [b'' [b''b' a'sb'']]. exists b''. split; [|done].
+  by etrans.
+Qed.
+
+(** ** [anywfo]: Direct sum of all [wfo]s
+  Note that [anywfo] itself can't belong to [wfo]
+  due to the universe hierarchy *)
+
+Record anywfo := Anywfo { anywfo_wfo : wfo; anywfo_val : anywfo_wfo }.
+
+(** [≼*!]: Reflexive order over [anywfo]s *)
+Definition anywfo_le (a b : anywfo) : Prop := a.(anywfo_val) ≼* b.(anywfo_val).
+Infix "≼*!" := anywfo_le (at level 70, no associativity) : nola_scope.
+Notation "(≼*!)" := anywfo_le (only parsing) : nola_scope.
+
+(** [≺*!]: Strict order over [anywfo]s *)
+Definition anywfo_lt (a b : anywfo) : Prop := a.(anywfo_val) ≺* b.(anywfo_val).
+Infix "≺*!" := anywfo_lt (at level 70, no associativity) : nola_scope.
+Notation "(≺*!)" := anywfo_lt (only parsing) : nola_scope.
+
+(** [≼*!] is reflexive *)
+#[export] Instance anywfo_le_refl : Reflexive anywfo_le.
+Proof. move=> a. apply wfo_sim_refl. Qed.
+
+(** [≼*!] is transitive *)
+#[export] Instance anywfo_le_trans : Transitive anywfo_le.
+Proof. move=> a b c. apply wfo_sim_trans. Qed.
+
+(** [≼*!] is a preorder *)
+#[export] Instance anywfo_le_preorder : PreOrder anywfo_le.
+Proof. split; apply _. Qed.
+
+(** [≺*!] is well-founded *)
+
+Lemma anywfo_lt_wf_pre {A : wfo} (a : A) :
+  Acc (≺) a → ∀{B : wfo} (b : B) , b ≼* a → Acc (≺*!) (Anywfo B b).
+Proof.
+  move: a. fix FIX 2=> a Acca B b /wfo_sim_unfold bsa. apply Acc_intro.
+  move=> [C c] [/=b' [csb' b'b]]. move: {bsa}(bsa b' b'b)=> [a' [a'a b'sa']].
+  eapply FIX; [exact (Acc_inv Acca a' a'a)|]. by eapply wfo_sim_trans.
+Qed.
+
+Lemma anywfo_lt_wf : wf (≺*!).
+Proof.
+  move=> [A a]. eapply anywfo_lt_wf_pre; [apply wfo_lt_wf|apply wfo_sim_refl].
+Qed.
